AczelSetTheory/Axioms.lean
@@ -45,3 +45,4 @@ import AczelSetTheory.Axioms.Induction
 import AczelSetTheory.Axioms.CartProd
 import AczelSetTheory.Axioms.Ordinal
 import AczelSetTheory.Axioms.OrdinalNat
+import AczelSetTheory.Axioms.Fintype
